Incorparating feedback, simplifying proofs
* Added all but three feedback elements from Implementation feedback
part 2
  - Haven't eliminated ret or live yet:
     Ret and live have different semantics, however it is possible to
simulate ret with live by \lambda x. live x, but it might prove
difficult  in proofs and to talk about it
  - May be requiring more examples, however the word count at the moment
is 11725 and still need a conclusion
  - Haven't played around with exact layouts of the semantics figures
yet.

* Proofs and semantics
  - Removed the inpair: it was a complete semantics duplication
  - Changed all of the proofs so that they work
  - "Simplified" a number of proofs by using copious amounts of
automatic proofsearch: less understandable by cases, much more succinct,
more resilient to slight changes.

* Added a makefile to build some stuff

mconbase.v
@@ -30,7 +30,6 @@ Inductive expr : Set :=
  | E_comp (e:expr)
  | E_live_expr (e:expr)
  | E_pair (e:expr) (e':expr)
- | E_inpair (e:expr) (e':expr)
  | E_proj1 (e:expr)
  | E_proj2 (e:expr)
  | E_fork (e:expr) (e':expr)
@@ -39,16 +38,9 @@ Inductive expr : Set :=
  | E_taggingright (e:expr)
  | E_case (e1:expr) (x1:value_name) (e2:expr) (x2:value_name) (e3:expr).
 
-Inductive selectopt : Set := 
- | SO_First : selectopt
- | SO_Second : selectopt.
-
 Inductive redlabel : Set := 
  | RL_tau : redlabel
  | RL_labelled (expr5:expr).
-
-CoInductive select : Set := 
- | S_Seq (o:selectopt) (s:select).
 
 Inductive G : Set := 
  | G_em : G
@@ -66,7 +58,6 @@ Fixpoint is_value_of_expr (e_5:expr) : Prop :=
   | (E_comp e) => False
   | (E_live_expr e) => (True)
   | (E_pair e e') => ((is_value_of_expr e) /\ (is_value_of_expr e'))
-  | (E_inpair e e') => False
   | (E_proj1 e) => False
   | (E_proj2 e) => False
   | (E_fork e e') => False
@@ -97,7 +88,6 @@ Fixpoint subst_expr (e_5:expr) (x_5:value_name) (e__6:expr) {struct e__6} : expr
   | (E_comp e) => E_comp (subst_expr e_5 x_5 e)
   | (E_live_expr e) => E_live_expr (subst_expr e_5 x_5 e)
   | (E_pair e e') => E_pair (subst_expr e_5 x_5 e) (subst_expr e_5 x_5 e')
-  | (E_inpair e e') => E_inpair (subst_expr e_5 x_5 e) (subst_expr e_5 x_5 e')
   | (E_proj1 e) => E_proj1 (subst_expr e_5 x_5 e)
   | (E_proj2 e) => E_proj2 (subst_expr e_5 x_5 e)
   | (E_fork e e') => E_fork (subst_expr e_5 x_5 e) (subst_expr e_5 x_5 e')
@@ -134,7 +124,6 @@ Fixpoint fv_expr (e_5:expr) : list value_name :=
   | (E_comp e) => ((fv_expr e))
   | (E_live_expr e) => ((fv_expr e))
   | (E_pair e e') => (app (fv_expr e) (fv_expr e'))
-  | (E_inpair e e') => (app (fv_expr e) (fv_expr e'))
   | (E_proj1 e) => ((fv_expr e))
   | (E_proj2 e) => ((fv_expr e))
   | (E_fork e e') => (app (fv_expr e) (fv_expr e'))
@@ -150,6 +139,14 @@ Definition fv_redlabel (rl5:redlabel) : list value_name :=
   | (RL_labelled expr5) => ((fv_expr expr5))
 end.
 
+
+Inductive selectopt : Set := 
+ | SO_First : selectopt
+ | SO_Second : selectopt.
+CoInductive select_h : Set := 
+| S_Seq (o:selectopt) (s:select_h). 
+
+Definition select : Set := select_h.
 (** definitions *)
 
 (* defns Jtype *)
@@ -158,7 +155,7 @@ Inductive VTSin : value_name -> typexpr -> G -> Prop :=    (* defn VTSin *)
      VTSin value_name5 typexpr5 (G_vn G5 value_name5 typexpr5)
  | VTSin_vn2 : forall (value_name5:value_name) (typexpr5:typexpr) (G5:G) (value_name':value_name) (typexpr':typexpr),
      VTSin value_name5 typexpr5 G5 ->
-      not(  value_name5 = value_name'  )  ->
+      ~(  value_name5 = value_name'  )  ->
      VTSin value_name5 typexpr5 (G_vn G5 value_name' typexpr')
 with Get : G -> expr -> typexpr -> Prop :=    (* defn Get *)
  | Get_ret : forall (G5:G) (e:expr) (t:typexpr),
@@ -170,10 +167,6 @@ with Get : G -> expr -> typexpr -> Prop :=    (* defn Get *)
      Get G5 (E_fork e e')  (TE_concurrent  (TE_sum  (TE_prod t1  (TE_concurrent t2) )   (TE_prod  (TE_concurrent t1)  t2) ) ) 
  | Get_unit : forall (G5:G),
      Get G5 E_unit TE_unit
- | Get_inpair : forall (G5:G) (e e':expr) (t1 t2:typexpr),
-     Get G5 e t1 ->
-     Get G5 e' t2 ->
-     Get G5 (E_inpair e e')  (TE_prod t1 t2) 
  | Get_proj1 : forall (G5:G) (e:expr) (t1 t2:typexpr),
      Get G5 e  (TE_prod t1 t2)  ->
      Get G5 (E_proj1 e) (TE_arrow  (TE_prod t1 t2)  t1)
@@ -236,11 +229,11 @@ Inductive JO_red : expr -> select -> redlabel -> expr -> Prop :=    (* defn red 
      JO_red (E_fork v e') s rl (E_fork v e'')
  | JO_red_forkmove1 : forall (e e':expr) (s:select) (rl:redlabel) (e'':expr),
      JO_red e s rl e'' ->
-     ~ (is_value_of_expr e')  ->
+      ~(is_value_of_expr( e' ))  ->
      JO_red (E_fork  (E_live_expr e)   (E_live_expr e') ) (S_Seq SO_First s) rl (E_fork  (E_live_expr e'')   (E_live_expr e') )
  | JO_red_forkmove2 : forall (e e':expr) (s:select) (rl:redlabel) (e'':expr),
      JO_red e' s rl e'' ->
-     ~ (is_value_of_expr e)  ->
+      ~(is_value_of_expr( e ))  ->
      JO_red (E_fork  (E_live_expr e)   (E_live_expr e') ) (S_Seq SO_Second s) rl (E_fork  (E_live_expr e)   (E_live_expr e'') )
  | JO_red_forkdeath1 : forall (v e:expr) (s:select),
      is_value_of_expr v ->
@@ -282,17 +275,6 @@ Inductive JO_red : expr -> select -> redlabel -> expr -> Prop :=    (* defn red 
      is_value_of_expr v ->
      JO_red e s rl e' ->
      JO_red (E_pair v e) s rl (E_pair v e')
- | JO_red_inpair : forall (v v':expr) (s:select),
-     is_value_of_expr v ->
-     is_value_of_expr v' ->
-     JO_red (E_inpair v v') s RL_tau (E_pair v v')
- | JO_red_inpair_eval1 : forall (e e':expr) (s:select) (rl:redlabel) (e'':expr),
-     JO_red e s rl e'' ->
-     JO_red (E_inpair e e') s rl (E_inpair e'' e')
- | JO_red_inpair_eval2 : forall (v e':expr) (s:select) (rl:redlabel) (e'':expr),
-     is_value_of_expr v ->
-     JO_red e' s rl e'' ->
-     JO_red (E_inpair v e') s rl (E_inpair v e'')
  | JO_red_proj1 : forall (v v':expr) (s:select),
      is_value_of_expr v ->
      is_value_of_expr v' ->
