Makefile
@@ -1,0 +1,31 @@
+#!/bin/bash
+# MC OCaml 
+
+FIGS=implOut gramDep
+DISSFOLDER=./Dissertation
+
+dissertation: figures fullSemantics
+
+figures: $(FIGS)
+
+implOut:
+	dot -Tps2 implOut.dot -o implOut.ps
+	epstopdf implOut.ps
+	rm -f $(DISSFOLDER)/implOut.pdf
+	cp implOut.pdf $(DISSFOLDER)
+gramDep:
+	rm -f mconbaseDep.dot
+	rm -f mconbaseDep.ps
+	rm -f $(DISSFOLDER)/mconbaseDep.pdf
+	ott -i mconbase.ott -dot mconbaseDep.dot
+	dot -Tps2 mconbaseDep.dot -o mconbaseDep.ps
+	epstopdf mconbaseDep.ps
+	cp mconbaseDep.pdf $(DISSFOLDER)
+
+fullSemantics:
+	rm -f mconbase.tex
+	rm -f mconbase_h.tex
+	rm -f mconbase.pdf
+	ott -i mconbase.ott -o mconbase_h.tex
+	sed -n -e :a -e '1,9!{P;N;D;};N;ba' mconbase_h.tex | sed '1,9d' > mconbase.tex
+
